HoareLogic/Sound_Basic.v
@@ -1,9 +1,11 @@
-Require Import Logic.MinimunLogic.LogicBase.
+Require Import Logic.GeneralLogic.Base.
+Require Import Logic.MinimunLogic.Syntax.
 Require Import Logic.PropositionalLogic.Syntax.
 Require Import Logic.SeparationLogic.Syntax.
-Require Import Logic.PropositionalLogic.KripkeSemantics.
-Require Import Logic.SeparationLogic.SeparationAlgebra.
-Require Import Logic.SeparationLogic.Semantics.
+Require Import Logic.PropositionalLogic.KripkeModel.
+Require Import Logic.SeparationLogic.Model.SeparationAlgebra.
+Require Import Logic.PropositionalLogic.Semantics.Kripke.
+Require Import Logic.SeparationLogic.Semantics.FlatSemantics.
 Require Import Logic.HoareLogic.ImperativeLanguage.
 Require Import Logic.HoareLogic.ProgramState.
 Require Import Logic.HoareLogic.BigStepSemantics.
@@ -25,7 +27,7 @@ Context {P: ProgrammingLanguage}
         {MD: Model}
         {BSS: BigStepSemantics P model}.
 
-Context {L: Language} {nL: NormalLanguage L} {pL: PropositionalLanguage L} {SL: SeparationLanguage L} {SM: Semantics L MD} {kiM: KripkeIntuitionisticModel model} {kiSM: KripkeIntuitionisticSemantics L MD tt SM}.
+Context {L: Language} {nL: NormalLanguage L} {pL: PropositionalLanguage L} {sL: SeparationLanguage L} {SM: Semantics L MD} {R: Relation model} {kiM: KripkeIntuitionisticModel model} {kiSM: KripkeIntuitionisticSemantics L MD (tt: @Kmodel MD (unit_kMD _)) SM}.
 
 Lemma hoare_consequence_partial_sound: forall c P1 P2 Q1 Q2,
   valid (AllModel _) (P2 --> P1) ->
